Break up the source into multiple files

LinearScan.v
@@ -6,864 +6,129 @@
 
     https://www.usenix.org/legacy/events/vee05/full_papers/p132-wimmer.pdf *)
 
-Require Import Coq.Arith.EqNat.
-Require Import Coq.Classes.EquivDec.
-Require Import Coq.Lists.List.
-Require Import Coq.Numbers.Natural.Peano.NPeano.
-Require Import Coq.Program.Basics.
+(* Require Import Coq.Arith.EqNat. *)
+(* Require Import Coq.Classes.EquivDec. *)
+(* Require Import Coq.Lists.List. *)
+(* Require Import Coq.Numbers.Natural.Peano.NPeano. *)
+(* Require Import Coq.Program.Basics. *)
 Require Import Coq.Program.Tactics.
-Require Import Coq.Logic.ProofIrrelevance.
-(* Require Import Coq.Sorting.Mergesort. *)
-(* Require Import Coq.Sorting.Sorting. *)
-Require Import Coq.Structures.Orders.
-Require Import Coq.Vectors.Fin.
-Require Import Recdef.
+(* Require Import Coq.Logic.ProofIrrelevance. *)
+(* (* Require Import Coq.Sorting.Mergesort. *) *)
+(* (* Require Import Coq.Sorting.Sorting. *) *)
+(* Require Import Coq.Structures.Orders. *)
+(* Require Import Coq.Vectors.Fin. *)
+(* Require Import Recdef. *)
+Require Import Interval.
+Require Import Range.
 Require Import Lib.
-Require String.
+Require Import ScanState.
 
-Module Import LN := ListNotations.
-(* jww (2014-09-25): I'll need to sort by the starting position of the
-   interval. *)
-(* Module Import MergeSort := Sort ??. *)
+Module MyMachine <: Machine.
 
-Open Scope string_scope.
-Open Scope nat_scope.
-Open Scope program_scope.
+Definition maxReg := 32.
+
+Lemma registers_exist : maxReg > 0.
+Proof. unfold maxReg. omega. Qed.
+
+End MyMachine.
+
+Module Import SS := MScanState MyMachine.
+(* Require String. *)
+
+(* Module Import LN := ListNotations. *)
+(* (* jww (2014-09-25): I'll need to sort by the starting position of the *)
+(*    interval, so a custom sorting predicate. *) *)
+(* (* Module Import MergeSort := Sort ??. *) *)
+
+(* Open Scope string_scope. *)
+(* Open Scope nat_scope. *)
+(* Open Scope program_scope. *)
 
 Generalizable All Variables.
-
-(****************************************************************************)
-
-(** * Core data types *)
-
-(** ** UsePos *)
-
-(** A "use position", or [UsePos], identifies an exact point in the
-    instruction stream where a particular variable is used.  If this usage
-    requires the use of a physical register, then [regReq] is [true] for that
-    use position. *)
-
-Record UsePos : Set := {
-  uloc   : nat;
-  regReq : bool
-}.
-
-(** ** Range *)
-
-(** The extent of a [Range] is the set of locations it ranges over.  By
-    summing the extent of a list of ranges, we have an idea of how much ground
-    is left to cover, and this gives us a notion of well-founded recursion for
-    iterating over intervals that may split as we examine them -- i.e., whose
-    total extent must decrease after each pass.
-
-    A Range is built up from a set of use positions, and defines the inclusive
-    range of those positions.  It can be extended, or split, but never shrunk.
-    Also, the non-empty list of use positions is not guaranteed to be in any
-    order, and overlapping use positions are accepted but only the most recent
-    one "wins". *)
-
-Record RangeDesc := {
-    rbeg : nat;
-    rend : nat;
-    ups  : NonEmpty UsePos;
-
-    range_nonempty : rbeg < rend         (* this comes in handy *)
-}.
-
-Inductive Range : RangeDesc -> Set :=
-  | R_Sing u :
-    Range {| rbeg := uloc u
-           ; rend := S (uloc u)
-           ; ups  := NE_Sing u
-           ; range_nonempty := le_n (S (uloc u))
-           |}
-
-  | R_Cons u x : Range x -> forall (H : uloc u < rbeg x),
-    Range {| rbeg := uloc u
-           ; rend := rend x
-           ; ups  := NE_Cons u (ups x)
-           ; range_nonempty := Lt.lt_trans _ _ _ H (range_nonempty x)
-           |}
-
-  | R_Extend x b' e' : Range x ->
-    Range {| rbeg := min b' (rbeg x)
-           ; rend := Peano.max e' (rend x)
-           ; ups  := ups x
-           ; range_nonempty := min_lt_max _ _ _ _ (range_nonempty x)
-           |}.
-
-Definition rangeExtent (x : RangeDesc) := rend x - rbeg x.
-
-Definition rangesIntersect (x y : RangeDesc) : bool :=
-  if rbeg x <? rbeg y
-  then rbeg y <? rend x
-  else rbeg x <? rend y.
-
-Definition rangesIntersectionPoint (x y : RangeDesc) : option nat :=
-  if rangesIntersect x y
-  then Some (min (rbeg x) (rbeg y))
-  else None.
-
-Definition anyRangeIntersects (is js : NonEmpty RangeDesc) : bool :=
-  fold_right
-    (fun r b => orb b (existsb (rangesIntersect r) (NE_to_list js)))
-    false (NE_to_list is).
-
-Fixpoint NE_fold_left {a b : Set} (f : a -> b -> a) (ne : NonEmpty b) (z : a) : a :=
-  match ne with
-    | NE_Sing x => f z x
-    | NE_Cons x xs => NE_fold_left f xs (f z x)
-  end.
-
-Definition firstIntersectionPoint (rd1 rd2 : NonEmpty RangeDesc)
-  : option nat :=
-  NE_fold_left
-    (fun acc rd =>
-       match acc with
-       | Some x => Some x
-       | None =>
-         NE_fold_left
-           (fun acc' rd' =>
-              match acc' with
-              | Some x => Some x
-              | None => rangesIntersectionPoint rd rd'
-              end) rd2 None
-       end) rd1 None.
-
-(** ** Interval *)
-
-(** A lifetime interval defines the lifetime of a variable.  It is defined as
-    a list of ranges "covered" by that variable in the low-level intermediate
-    representation (LIR).  Gaps in the list of ranges are called "lifetime
-    holes".
-
-    A lifetime is not necessarily only the distance that a variable is first
-    and last used.  The lifetime of a variable used in a loop extends to the
-    whole loop, for example, even if it is only used at the very end.  In this
-    sense, coverage takes into account code flow, or what ranges would map to
-    if all loops were unrolled, and then rolled back keeping track of
-    coverage.
-
-    Use positions are actual instructions where a variable is read from or
-    written to, and whether it is required to be in a register at that
-    point. *)
-
-(** If for some reason we cannot assign a single register for all ranges, then
-    the interval is split into two or more intervals, so each interval can be
-    assigned its own register. *)
-
-Record IntervalDesc := {
-    ibeg : nat;
-    iend : nat;
-    rds  : NonEmpty RangeDesc;
-
-    (** Caching this property comes in handy, as it can be tricky to determine
-        it by reduction in some cases. *)
-    interval_nonempty : ibeg < iend
-}.
-
-Inductive Interval : IntervalDesc -> Set :=
-  | I_Sing : forall x, Range x ->
-      Interval {| ibeg := rbeg x
-                ; iend := rend x
-                ; rds  := NE_Sing x
-                ; interval_nonempty := range_nonempty x
-                |}
-
-  | I_Cons1 : forall x y ib ie ne,
-      Interval {| ibeg := ib; iend := ie; rds := NE_Sing y;
-                  interval_nonempty := ne |}
-        -> Range x -> forall (H : rend x <= ib),
-      Interval {| ibeg := rbeg x
-                ; iend := ie
-                ; rds  := NE_Cons x (NE_Sing y)
-                ; interval_nonempty := lt_le_shuffle (range_nonempty x) H ne
-                |}
-
-  | I_Consn : forall x y xs ib ie ne,
-      Interval {| ibeg := ib; iend := ie; rds := NE_Cons y xs;
-                  interval_nonempty := ne |}
-        -> Range x -> forall (H : rend x <= ib),
-      Interval {| ibeg := rbeg x
-                ; iend := ie
-                ; rds  := NE_Cons x (NE_Cons y xs)
-                ; interval_nonempty := lt_le_shuffle (range_nonempty x) H ne
-                |}.
-
-Definition intervalStart `(i : Interval d) : nat := ibeg d.
-Definition intervalEnd   `(i : Interval d) : nat := iend d.
-
-Definition intervalCoversPos `(i : Interval rs) (pos : nat) : bool :=
-  andb (intervalStart i <=? pos) (pos <? intervalEnd i).
-
-Definition intervalExtent `(i : Interval rs) :=
-  intervalEnd i - intervalStart i.
-
-Lemma Interval_nonempty : forall `(i : Interval rs),
-  intervalStart i < intervalEnd i.
-Proof.
-  intros. unfold intervalStart, intervalEnd.
-  induction i; simpl in *;
-  induction r; simpl in *; min_max.
-Qed.
-
-Lemma Interval_extent_nonzero : forall `(i : Interval rs),
-  intervalExtent i > 0.
-Proof.
-  intros.
-  unfold intervalExtent.
-  pose (Interval_nonempty i).
-  apply lt_minus in l. assumption.
-Qed.
-
-(****************************************************************************)
-
-(** * Main algorithm *)
-
-Section Allocator.
-
-Variable maxReg : nat.          (* max number of registers *)
-
-Hypothesis registers_exist : maxReg > 0.
-
-Definition VirtReg := nat.
-Definition PhysReg := fin maxReg.
-
-(** ** ScanState *)
-
-(** A [ScanState] is always relative to a current position (pos) as we move
-    through the sequentialized instruction stream over which registers are
-    allocated.. *)
-
-Record ScanStateDesc := {
-    nextInterval : nat;
-    IntervalId   := fin nextInterval;
-
-    unhandled : list IntervalId;   (* starts after pos *)
-    active    : list IntervalId;   (* ranges over pos *)
-    inactive  : list IntervalId;   (* falls in lifetime hole *)
-    handled   : list IntervalId;   (* ends before pos *)
-
-    getInterval  : IntervalId -> { d : IntervalDesc & Interval d };
-    assignments  : IntervalId -> option PhysReg;
-
-    (* jww (2014-09-25): These restricting lemmas should be added back once
-       everything is functional. *)
-    (* unhandled_sorted : StronglySorted cmp_le unhandled; *)
-
-    all_state_lists  := unhandled ++ active ++ inactive ++ handled;
-    lists_are_unique : NoDup all_state_lists
-}.
-
-Lemma lt_sub : forall n m, n < m -> { p : nat | p = m - n }.
-Proof. intros. exists (m - n). reflexivity. Defined.
-
-Definition transportId `(H : nextInterval st <= nextInterval st')
-  (x : IntervalId st) : IntervalId st'.
-Proof.
-  apply Compare_dec.le_lt_eq_dec in H.
-  destruct H.
-    destruct st. destruct st'.
-    unfold IntervalId0, IntervalId1 in *.
-    unfold IntervalId in *. simpl in *.
-    pose proof l.
-    apply lt_sub in H.
-    destruct H.
-    symmetry in e.
-    apply Nat.add_sub_eq_nz in e.
-      rewrite Plus.plus_comm in e.
-      rewrite <- e.
-      apply (R x0 x).
-    subst. omega.
-  unfold IntervalId in *.
-  rewrite <- e.
-  assumption.
-Defined.
-
-Lemma move_unhandled_to_active : forall n (x : fin n) unh act inact hnd,
-  NoDup ((x :: unh) ++ act ++ inact ++ hnd)
-    -> NoDup (unh ++ (x :: act) ++ inact ++ hnd).
-Proof.
-  intros. rewrite <- app_comm_cons.
-  apply NoDup_app_cons. assumption.
-Qed.
-
-Lemma move_active_to_inactive : forall sd x,
-  NoDup (unhandled sd ++ active sd ++ inactive sd ++ handled sd)
-    -> In x (active sd)
-    -> NoDup (unhandled sd ++ remove cmp_eq_dec x (active sd) ++
-              (x :: inactive sd) ++ handled sd).
-Proof.
-  intros.
-  apply NoDup_swap.
-  rewrite <- app_assoc.
-  rewrite <- app_assoc.
-  apply NoDup_juggle.
-  rewrite app_assoc.
-  rewrite app_assoc.
-  apply NoDup_swap.
-  rewrite <- app_assoc.
-  assumption.
-  apply H0.
-Qed.
-
-Lemma move_active_to_handled : forall sd x,
-  NoDup (unhandled sd ++ active sd ++ inactive sd ++ handled sd)
-    -> In x (active sd)
-    -> NoDup (unhandled sd ++ remove cmp_eq_dec x (active sd) ++
-              inactive sd ++ x :: handled sd).
-Proof.
-  intros.
-  apply NoDup_swap.
-  rewrite <- app_assoc.
-  rewrite <- app_assoc.
-  apply NoDup_swap2.
-  rewrite <- app_assoc.
-  apply NoDup_juggle.
-  rewrite app_assoc.
-  apply NoDup_swap2.
-  rewrite app_assoc.
-  apply NoDup_swap.
-  rewrite <- app_assoc.
-  rewrite app_assoc.
-  apply NoDup_swap2.
-  rewrite <- app_assoc.
-  assumption.
-  apply H0.
-Qed.
-
-Lemma move_inactive_to_active : forall sd x,
-  NoDup (unhandled sd ++ active sd ++ inactive sd ++ handled sd)
-    -> In x (inactive sd)
-    -> NoDup (unhandled sd ++ x :: active sd ++
-              remove cmp_eq_dec x (inactive sd) ++ handled sd).
-Proof.
-  intros.
-  rewrite app_comm_cons.
-  apply NoDup_swap.
-  rewrite <- app_assoc.
-  apply NoDup_swap.
-  repeat rewrite <- app_assoc.
-  rewrite (app_assoc (handled sd)).
-  apply NoDup_swap2.
-  apply NoDup_juggle.
-  repeat rewrite app_assoc.
-  apply NoDup_swap.
-  rewrite <- app_assoc.
-  apply NoDup_swap2.
-  rewrite <- app_assoc.
-  rewrite app_assoc.
-  apply NoDup_swap2.
-  rewrite <- app_assoc.
-  assumption.
-  apply H0.
-Qed.
-
-Lemma move_inactive_to_handled : forall sd x,
-  NoDup (unhandled sd ++ active sd ++ inactive sd ++ handled sd)
-    -> In x (inactive sd)
-    -> NoDup (unhandled sd ++ active sd ++
-              remove cmp_eq_dec x (inactive sd) ++ x :: handled sd).
-Proof.
-  intros.
-  rewrite (app_assoc (unhandled sd)).
-  apply NoDup_swap.
-  repeat rewrite <- app_assoc.
-  apply NoDup_juggle.
-  rewrite (app_assoc (inactive sd)).
-  apply NoDup_swap.
-  repeat rewrite <- app_assoc.
-  assumption.
-  apply H0.
-Qed.
-
-(** The [ScanState] inductive data type describes the allowable state
-    transitions that can be applied to a [ScanStateDesc] value.
-
-    In essence there are five mutating operations:
-
-    1. Create a new unhandled interval.  This can occur for two reasons:
-
-       a. Adding a new interval to be considered before the linear scan
-          algorithm has started.
-       b. Splitting the current interval, which pushes back its "pieces" as
-          new unhandled intervals.
-
-    2. Remove the first unhandled interval.  This happens when we remove it in
-       order to make it the new current interval.
-
-    3. Add the current interval to the active list.
-
-    4. Move an item from the active list to the inactive or handled lists.
-
-    5. Move an item from the inactive list to the active or handled lists. *)
-
-Inductive ScanState : ScanStateDesc -> Set :=
-  | ScanState_nil :
-    ScanState
-      {| nextInterval     := 0
-       ; unhandled        := nil
-       ; active           := nil
-       ; inactive         := nil
-       ; handled          := nil
-       ; getInterval      := fin_contra
-       ; assignments      := fin_contra
-       (* ; unhandled_sorted := LSorted_nil _ *)
-       ; lists_are_unique := NoDup_nil _
-       |}
-
-  | ScanState_newUnhandled
-      ni unh (* unhsort *) act inact hnd geti assgn lau :
-    forall `(i : Interval d),
-    ScanState
-      {| nextInterval     := ni
-       ; unhandled        := unh
-       ; active           := act
-       ; inactive         := inact
-       ; handled          := hnd
-       ; getInterval      := geti
-       ; assignments      := assgn
-       (* ; unhandled_sorted := unhsort *)
-       ; lists_are_unique := lau
-       |} ->
-    forall newi (H : newi = last_fin_from_nat ni),
-    ScanState
-      {| nextInterval     := S ni
-       ; unhandled        := newi :: map fin_expand unh
-       ; active           := map fin_expand act
-       ; inactive         := map fin_expand inact
-       ; handled          := map fin_expand hnd
-       ; getInterval      :=
-         fun n => match cmp_eq_dec n newi with
-                  | left _ => existT _ d i
-                  | right Hn => geti (fin_safe_reduce n (rew_in_not_eq H Hn))
-                  end
-       ; assignments      :=
-         fun n => match cmp_eq_dec n newi with
-                  | left _ => None
-                  | right Hn => assgn (fin_safe_reduce n (rew_in_not_eq H Hn))
-                  end
-       (* ; unhandled_sorted := unhsort *)
-       ; lists_are_unique := map_fin_expand_rewrite (NoDup_fin_cons _ _ lau H)
-       |}
-
-  | ScanState_moveUnhandledToActive
-      ni unh (* unhsort *) act inact hnd geti assgn x reg :
-    forall lau : NoDup ((x :: unh) ++ act ++ inact ++ hnd),
-    ScanState
-      {| nextInterval     := ni
-       ; unhandled        := x :: unh
-       ; active           := act
-       ; inactive         := inact
-       ; handled          := hnd
-       ; getInterval      := geti
-       ; assignments      := assgn
-       (* ; unhandled_sorted := unhandled_sorted sd *)
-       ; lists_are_unique := lau
-       |} ->
-    ScanState
-      {| nextInterval     := ni
-       ; unhandled        := unh
-       ; active           := x :: act
-       ; inactive         := inact
-       ; handled          := hnd
-       ; getInterval      := geti
-       ; assignments      := fun i => if cmp_eq_dec i x
-                                      then Some reg
-                                      else assgn i
-       (* ; unhandled_sorted := unhandled_sorted sd *)
-       ; lists_are_unique := move_unhandled_to_active _ x unh act inact hnd lau
-       |}
-
-  | ScanState_moveActiveToInactive sd x :
-    ScanState sd -> forall (H : In x (active sd)),
-    ScanState
-      {| nextInterval     := nextInterval sd
-       ; unhandled        := unhandled sd
-       ; active           := remove cmp_eq_dec x (active sd)
-       ; inactive         := x :: inactive sd
-       ; handled          := handled sd
-       ; getInterval      := getInterval sd
-       ; assignments      := assignments sd
-       (* ; unhandled_sorted := unhandled_sorted sd *)
-       ; lists_are_unique :=
-         move_active_to_inactive sd x (lists_are_unique sd) H
-       |}
-
-  | ScanState_moveActiveToHandled sd x :
-    ScanState sd -> forall (H : In x (active sd)),
-    ScanState
-      {| nextInterval     := nextInterval sd
-       ; unhandled        := unhandled sd
-       ; active           := remove cmp_eq_dec x (active sd)
-       ; inactive         := inactive sd
-       ; handled          := x :: handled sd
-       ; getInterval      := getInterval sd
-       ; assignments      := assignments sd
-       (* ; unhandled_sorted := unhandled_sorted sd *)
-       ; lists_are_unique :=
-         move_active_to_handled sd x (lists_are_unique sd) H
-       |}
-
-  | ScanState_moveInactiveToActive sd x :
-    ScanState sd -> forall (H : In x (inactive sd)),
-    ScanState
-      {| nextInterval     := nextInterval sd
-       ; unhandled        := unhandled sd
-       ; active           := x :: active sd
-       ; inactive         := remove cmp_eq_dec x (inactive sd)
-       ; handled          := handled sd
-       ; getInterval      := getInterval sd
-       ; assignments      := assignments sd
-       (* ; unhandled_sorted := unhandled_sorted sd *)
-       ; lists_are_unique :=
-         move_inactive_to_active sd x (lists_are_unique sd) H
-       |}
-
-  | ScanState_moveInactiveToHandled sd x :
-    ScanState sd -> forall (H : In x (inactive sd)),
-    ScanState
-      {| nextInterval     := nextInterval sd
-       ; unhandled        := unhandled sd
-       ; active           := active sd
-       ; inactive         := remove cmp_eq_dec x (inactive sd)
-       ; handled          := x :: handled sd
-       ; getInterval      := getInterval sd
-       ; assignments      := assignments sd
-       (* ; unhandled_sorted := unhandled_sorted sd *)
-       ; lists_are_unique :=
-         move_inactive_to_handled sd x (lists_are_unique sd) H
-       |}.
-
-Tactic Notation "ScanState_cases" tactic(first) ident(c) :=
-  first;
-  [ Case_aux c "ScanState_nil"
-  | Case_aux c "ScanState_newUnhandled"
-  | Case_aux c "ScanState_moveUnhandledToActive"
-  | Case_aux c "ScanState_moveActiveToInactive"
-  | Case_aux c "ScanState_moveActiveToHandled"
-  | Case_aux c "ScanState_moveInactiveToActive"
-  | Case_aux c "ScanState_moveInactiveToHandled"
-  ].
-
-Ltac cmp_reflexive :=
-  match goal with
-    [ |- context [match cmp_eq_dec ?X ?X with _ => _ end] ] =>
-      assert (cmp_eq_dec X X = left eq_refl) as Hrcmp
-        by (intros; destruct (cmp_eq_dec X X);
-              [ f_equal; apply proof_irrelevance
-              | intuition ]);
-      rewrite Hrcmp in *; clear Hrcmp; simpl in *
-  end.
-
-Definition unhandledExtent `(sd : ScanStateDesc) : nat :=
-  match unhandled sd with
-  | nil => 0
-  | [i] => intervalExtent (projT2 (getInterval sd i))
-  | xs  =>
-    let f n x := n + intervalExtent (projT2 (getInterval sd x)) in
-    fold_left f xs 0
-  end.
-
-Theorem ScanState_unhandledExtent `(st : ScanState sd) :
-  let unh := unhandled sd in
-  let ue  := unhandledExtent sd in
-  match unh with
-  | nil    => ue = 0
-  | [i]    => ue = intervalExtent (projT2 (getInterval sd i))
-  | i :: _ => ue > intervalExtent (projT2 (getInterval sd i))
-  end.
-Proof.
-  destruct sd.
-  destruct unhandled0 eqn:Heqe;
-  unfold unhandledExtent; simpl.
-    reflexivity.
-  destruct l eqn:Heqe2; simpl.
-    reflexivity.
-  apply fold_gt.
-  pose (Interval_extent_nonzero (projT2 (getInterval0 i0))).
-  omega.
-Defined.
-
-Lemma unhandledExtent_cons
-  : forall ni i (unh : list (fin ni)) geti assgn assgn'
-           (act act' inact inact' hnd hnd' : list (fin ni))
-           (lau : NoDup (unh ++ act ++ inact ++ hnd))
-           (lau' : NoDup ((i :: unh) ++ act' ++ inact' ++ hnd')),
-  unhandledExtent
-    {| nextInterval     := ni
-     ; unhandled        := unh
-     ; active           := act
-     ; inactive         := inact
-     ; handled          := hnd
-     ; getInterval      := geti
-     ; assignments      := assgn
-     ; lists_are_unique := lau
-     |} <
-  unhandledExtent
-    {| nextInterval     := ni
-     ; unhandled        := i :: unh
-     ; active           := act'
-     ; inactive         := inact'
-     ; handled          := hnd'
-     ; getInterval      := geti
-     ; assignments      := assgn'
-     ; lists_are_unique := lau'
-     |}.
-Proof.
-  intros.
-  induction unh; unfold unhandledExtent; simpl;
-  pose (Interval_extent_nonzero (projT2 (geti i))). omega.
-  destruct unh; simpl. omega.
-  apply fold_fold_lt. omega.
-Qed.
-
-Record ScanStateCursor (sd : ScanStateDesc) := {
-    curState    : ScanState sd;
-    curExists   : length (unhandled sd) > 0;
-
-    curId       := safe_hd (unhandled sd) curExists;
-
-    curIntDesc  : IntervalDesc;
-    curInterval := projT2 (getInterval sd curId);
-
-    curPosition := intervalStart curInterval
-}.
-
-Arguments curState    {sd} _.
-Arguments curExists   {sd} _.
-Arguments curId       {sd} _.
-Arguments curIntDesc  {sd} _.
-Arguments curInterval {sd} _.
-Arguments curPosition {sd} _.
-
-Record NextScanState (P : ScanStateDesc -> Prop) : Type := {
-    nextDesc   : ScanStateDesc;
-    nextState  : ScanState nextDesc;
-    morphProof : P nextDesc
-}.
-
-Arguments Build_NextScanState [P] _ _ _.
-
-Arguments nextDesc   [P] _.
-Arguments nextState  [P] _.
-Arguments morphProof [P] _.
-
-Definition NextState `(cur : ScanStateCursor sd) P := NextScanState (P sd).
-
-Definition NextStateDep  `(cur : ScanStateCursor sd) P Q :=
-  { x : NextScanState (P sd) & Q x }.
-
-Definition NextStateWith `(cur : ScanStateCursor sd) P A :=
-  (A * NextScanState (P sd))%type.
-
-Definition NextScanState_transitivity
-  {P : ScanStateDesc -> ScanStateDesc -> Prop} `{Transitive _ P}
-  `(n : NextScanState (P sd0)) `(o : NextScanState (P (nextDesc n)))
-  : NextScanState (P sd0).
-  destruct n. destruct o.
-  simpl in *.
-  rapply Build_NextScanState.
-    apply nextState1.
-  transitivity nextDesc0; assumption.
-Defined.
-
-(** ** SSMorph *)
-
-(** A [SSMorph] is a relation describe a lawful transition between two
-    states.  It is a [PreOrder] relation. *)
-
-Record SSMorph (sd1 sd2 : ScanStateDesc) : Prop := {
-    next_interval_increases : nextInterval sd1     <= nextInterval sd2;
-    total_extent_decreases  : unhandledExtent sd2  <= unhandledExtent sd1;
-    handled_count_increases : length (handled sd1) <= length (handled sd2)
-}.
-
-Arguments next_interval_increases [sd1 sd2] _.
-Arguments total_extent_decreases  [sd1 sd2] _.
-Arguments handled_count_increases [sd1 sd2] _.
-
-Definition newSSMorph (s : ScanStateDesc) : SSMorph s s.
-Proof. constructor; auto. Defined.
-
-Program Instance SSMorph_PO : PreOrder SSMorph.
-Obligation 1. constructor; auto. Defined.
-Obligation 2.
-  constructor; destruct H; destruct H0.
-  transitivity (nextInterval y); auto.
-  transitivity (unhandledExtent y); auto.
-  transitivity (length (handled y)); auto.
-Defined.
-
-Record SSMorphLen (sd1 sd2 : ScanStateDesc) : Prop := {
-    len_is_SSMorph :> SSMorph sd1 sd2;
-
-    unhandled_nonempty :
-      length (unhandled sd1) > 0 -> length (unhandled sd2) > 0
-}.
-
-Definition newSSMorphLen (s : ScanStateDesc) : SSMorphLen s s.
-Proof. intros. constructor; auto. constructor; auto. Defined.
-
-Record SSMorphSt (sd1 sd2 : ScanStateDesc) : Prop := {
-    st_is_SSMorph :> SSMorph sd1 sd2;
-
-    total_extent_measurably_decreases :
-      unhandledExtent sd2 < unhandledExtent sd1
-}.
-
-Program Instance SSMorphSt_Trans : Transitive SSMorphSt.
-Obligation 1.
-  constructor.
-    destruct H. destruct H0.
-    transitivity y; assumption.
-  inversion H. inversion H0.
-  destruct total_extent_measurably_decreases1. omega.
-  destruct total_extent_measurably_decreases0. omega.
-  right. omega.
-Qed.
-
-Lemma ScanState_unhandledExtent_nonzero `(st : ScanState sd) :
-  length (unhandled sd) > 0 <-> unhandledExtent sd > 0.
-Proof.
-  intros.
-  ScanState_cases (induction st) Case; simpl in *.
-  - Case "ScanState_nil".
-    split; intros; inversion H.
-  - Case "ScanState_newUnhandled".
-    pose (Interval_extent_nonzero i).
-    destruct unh eqn:Heqe;
-    unfold unhandledExtent; simpl.
-      split; intros; try cmp_reflexive; auto.
-    destruct l eqn:Heqe2; simpl.
-      split; intros; try cmp_reflexive; auto. omega.
-    split; intros.
-      apply fold_gt.
-      cmp_reflexive. omega.
-    apply Gt.gt_Sn_O.
-  - Case "ScanState_moveUnhandledToActive".
-    apply ScanState_unhandledExtent in st.
-    rename st into i. simpl in *.
-    destruct unh eqn:Heqe.
-      split; intros. inversion H. auto.
-    unfold unhandledExtent; simpl.
-    destruct l eqn:Heqe2; simpl.
-      split; intros.
-      apply Interval_extent_nonzero.
-      auto.
-    split; intros.
-      apply fold_gt.
-      pose (Interval_extent_nonzero (projT2 (geti f))).
-      omega.
-    omega.
-  - Case "ScanState_moveActiveToInactive".  apply IHst.
-  - Case "ScanState_moveActiveToHandled".   apply IHst.
-  - Case "ScanState_moveInactiveToActive".  apply IHst.
-  - Case "ScanState_moveInactiveToHandled". apply IHst.
-Qed.
-
-Definition moveActiveToHandled `(st : ScanState sd) (x : IntervalId sd)
-  (H : In x (active sd)) : NextScanState (SSMorphLen sd).
-Proof.
-  pose (ScanState_moveActiveToInactive sd x st H). eexists. apply s.
-  destruct sd. simpl.
-  rapply Build_SSMorphLen; auto.
-  rapply Build_SSMorph; auto.
-Defined.
-
-Definition moveActiveToInactive `(st : ScanState sd) (x : IntervalId sd)
-  (H : In x (active sd)) : NextScanState (SSMorphLen sd).
-Proof.
-  pose (ScanState_moveActiveToInactive sd x st H). eexists. apply s.
-  destruct sd. simpl.
-  rapply Build_SSMorphLen; auto.
-  rapply Build_SSMorph; auto.
-Defined.
-
-Definition moveInactiveToActive `(st : ScanState sd) (x : IntervalId sd)
-  (H : In x (inactive sd)) : NextScanState (SSMorphLen sd).
-Proof.
-  pose (ScanState_moveInactiveToActive sd x st H). eexists. apply s.
-  destruct sd. simpl.
-  rapply Build_SSMorphLen; auto.
-  rapply Build_SSMorph; auto.
-Defined.
-
-Definition moveInactiveToHandled `(st : ScanState sd) (x : IntervalId sd)
-  (H : In x (inactive sd)) : NextScanState (SSMorphLen sd).
-Proof.
-  pose (ScanState_moveInactiveToHandled sd x st H). eexists. apply s.
-  destruct sd. simpl.
-  rapply Build_SSMorphLen; auto.
-  rapply Build_SSMorph; auto.
-  apply Le.le_n_Sn.
-Defined.
-
-Definition moveUnhandledToActive `(st : ScanState sd) (reg : PhysReg)
-  (H : length (unhandled sd) > 0) : NextScanState (SSMorphSt sd).
-Proof.
-  destruct sd.
-  destruct unhandled0; simpl in *. omega.
-  pose (ScanState_moveUnhandledToActive
-          nextInterval0 unhandled0
-          (* unhsort *)
-          active0 inactive0 handled0
-          getInterval0 assignments0
-          i reg lists_are_unique0).
-  eexists. apply s. apply st.
-  pose (unhandledExtent_cons nextInterval0 i unhandled0 getInterval0
-         (fun i0 : fin nextInterval0 =>
-            if cmp_eq_dec i0 i
-            then Some reg
-            else assignments0 i0) assignments0
-         (i :: active0) active0 inactive0 inactive0 handled0 handled0
-         (move_unhandled_to_active _ i unhandled0 active0 inactive0 handled0
-            lists_are_unique0) lists_are_unique0)
-    as ue_cons.
-  rapply Build_SSMorphSt; auto.
-  rapply Build_SSMorph; auto.
-  apply (Lt.lt_le_weak _ _ ue_cons).
-Defined.
-
-(** ** Main functions *)
 
 Definition nextIntersectionWith
   `(Interval xd) `(it : IntervalId sd) : option nat :=
   let itval := getInterval sd it in
   firstIntersectionPoint (rds (projT1 itval)) (rds xd).
 
-Definition getRegisterIndex `(st : ScanState sd) (k : IntervalId sd -> option nat)
-  (z : PhysReg -> option nat) (is : list (IntervalId sd))
-  : PhysReg -> option nat :=
+(** Given a function from intervals to indices ([intervalIndex]), and a
+    default function from registers to indices ([registerIndex]), build a
+    complete function from registers to indices by looking up the given
+    register in the list of assignments, finding the first interval it has
+    been assigned to, and then using [intervalIndex] to find the index, if
+    any. *)
+
+Definition getRegisterIndex `(st : ScanState sd)
+  (intervalIndex : IntervalId sd -> option nat)
+  (registerIndex : PhysReg -> option nat)
+  (intervals : list (IntervalId sd)) : PhysReg -> option nat :=
   fold_right
     (fun x f => fun r =>
        match assignments sd x with
        | None => f r
-       | Some a => if cmp_eq_dec a r then k x else f r
-       end) z is.
+       | Some a => if cmp_eq_dec a r then intervalIndex x else f r
+       end) registerIndex intervals.
 
-Function findRegister (freeUntilPos : PhysReg -> option nat) (reg : PhysReg)
-  {measure fin_to_nat reg} : (PhysReg * option nat)%type :=
-  match freeUntilPos reg with
-  | None => (reg, None)
+(** Given a function from registers to indices ([registerIndex]), and a
+    starting register [start] (the highest register to be considered), look
+    through the registers from highest to lowest to find the one with the
+    highest associated index, where [None] counts as infinitely high (i.e.,
+    unassociated). *)
+
+Function findRegister (registerIndex : PhysReg -> option nat)
+  (start : PhysReg) {measure fin_to_nat start}
+  : (PhysReg * option nat)%type :=
+  match registerIndex start with
+  | None => (start, None)
   | Some pos =>
-      match pred_fin reg with
-      | None => (reg, Some pos)
+      match pred_fin start with
+      | None => (start, Some pos)
       | Some nreg =>
-          match findRegister freeUntilPos nreg with
-          | (reg', None) => (reg', None)
-          | (reg', Some pos') =>
+          match findRegister registerIndex nreg with
+          | (reg, None) => (reg, None)
+          | (reg, Some pos') =>
               if pos <? pos'
-              then (reg', Some pos')
-              else (reg,  Some pos)
+              then (reg, Some pos')
+              else (reg, Some pos)
           end
       end
   end.
 Proof. intros; apply pred_fin_lt; assumption. Qed.
 
-Definition splitInterval `(cur : ScanStateCursor sd) (before : nat)
-  : NextState cur SSMorphSt :=
+(** Split the current interval before position [before].  This must succeed,
+    which means there must be use positions within the interval prior to
+    [before].  If [before] is [None], then splitting is done before the first
+    use position that does not require a register.
+
+    The resulting intervals are sorted back into the unhandled
+    list, so that the next interval to be processed may not be the remainder
+    of the split interval. *)
+
+Definition splitInterval `(cur : ScanStateCursor sd) (before : option nat)
+  : NextState cur SSMorphStLen :=
+  (* jww (2014-09-26): NYI *)
   Build_NextScanState sd (curState cur) undefined.
+
+Definition cursorFromMorphLen `(cur : ScanStateCursor sd)
+  `(n : NextState cur SSMorphLen) : ScanStateCursor (nextDesc n).
+Proof.
+  destruct sd. destruct cur. simpl in *.
+  rapply Build_ScanStateCursor;
+  destruct n; simpl in *.
+  - apply nextState0.
+  - destruct morphProof0.
+    destruct nextDesc0.
+    simpl in *. omega.
+  - auto.
+Defined.
+
+Definition cursorFromMorphStLen `(cur : ScanStateCursor sd)
+  `(n : NextState cur SSMorphStLen) : ScanStateCursor (nextDesc n) :=
+  cursorFromMorphLen cur
+    {| nextDesc   := nextDesc n
+     ; nextState  := nextState n
+     ; morphProof := stlen_is_SSMorphLen _ _ (morphProof n)
+     |}.
 
 (** If [tryAllocateFreeReg] fails to allocate a register, the [ScanState] is
     left unchanged.  If it succeeds, or is forced to split [current], then a
@@ -880,56 +145,87 @@ Definition tryAllocateFreeReg `(cur : ScanStateCursor sd)
        freeUntilPos[it.reg] = 0
      for each interval it in inactive intersecting with current do
        freeUntilPos[it.reg] = next intersection of it with current *)
-  let st := curState cur in
+  let st      := curState cur in
   let current := curInterval cur in
+
   let freeUntilPos' :=
-        getRegisterIndex st (const (Some 0)) (const None) (active sd) in
+      getRegisterIndex st (const (Some 0)) (const None) (active sd) in
+  let intersectingIntervals :=
+        filter (fun x => anyRangeIntersects
+                           (rds (curIntDesc cur))
+                           (rds (projT1 (getInterval sd x))))
+               (inactive sd) in
   let freeUntilPos :=
-        getRegisterIndex st (nextIntersectionWith current)
-                         freeUntilPos' (inactive sd) in
+      getRegisterIndex st (nextIntersectionWith current) freeUntilPos'
+                       intersectingIntervals in
 
   (* reg = register with highest freeUntilPos *)
   let lastReg     := ultimate_from_nat maxReg registers_exist in
   let (reg, mres) := findRegister freeUntilPos lastReg in
-  let result      := moveUnhandledToActive st reg (curExists cur) in
+  let default     := moveUnhandledToActive cur reg in
 
-  (* [mres] indicates the highest use position of the indicated register,
-     which is the furthest available. *)
+  (* [mres] indicates the highest use position of the found register *)
   match mres with
-  | None => Some result
+  | None => Some default
   | Some n =>
-      (* if freeUntilPos[reg] = 0 then
-           // no register available without spilling
-           allocation failed
-         else if current ends before freeUntilPos[reg] then
-           // register available for the whole interval
-           current.reg = reg
-         else
-           // register available for the first part of the interval
-           current.reg = reg
-           split current before freeUntilPos[reg] *)
-      if beq_nat n 0
-      then None
-      else if ltb (intervalEnd current) n
-           then Some result
-           else None            (* jww (2014-09-12): NYI *)
+    (* if freeUntilPos[reg] = 0 then
+         // no register available without spilling
+         allocation failed
+       else if current ends before freeUntilPos[reg] then
+         // register available for the whole interval
+         current.reg = reg
+       else
+         // register available for the first part of the interval
+         current.reg = reg
+         split current before freeUntilPos[reg] *)
+    if beq_nat n 0
+    then None
+    else Some
+      (if ltb (intervalEnd current) n
+       then default
+       else moveUnhandledToActive
+              (cursorFromMorphStLen cur (splitInterval cur (Some n))) reg)
   end.
 
+Definition nextUseAfter (pos : nat) `(curId : IntervalId desc) : option nat.
+  (* jww (2014-09-26): NYI *)
+Admitted.
+
+Definition assignSpillSlotToCurrent `(cur : ScanStateCursor sd)
+  : NextScanState (SSMorphLen sd).
+  (* jww (2014-09-26): NYI *)
+Admitted.
+
 (** If [allocateBlockedReg] fails, it's possible no register was assigned and
-    that the only outcome was to split one or more intervals.  This is why the
-    type differs from [tryAllocateFreeReg], since in all cases the final state
-    is changed. *)
+    that the only outcome was to split one or more intervals.  In either case,
+    the change to the [ScanState] must be a productive one. *)
 Definition allocateBlockedReg `(cur : ScanStateCursor sd)
   : NextState cur SSMorphSt :=
-  (* set nextUsePos of all physical registers to maxInt *)
-
-  (* for each interval it in active do
+  (* set nextUsePos of all physical registers to maxInt
+     for each interval it in active do
        nextUsePos[it.reg] = next use of it after start of current
      for each interval it in inactive intersecting with current do
        nextUsePos[it.reg] = next use of it after start of current *)
+  let st      := curState cur in
+  let current := curInterval cur in
+  let pos     := curPosition cur in
 
-  (* reg = register with highest nextUsePos
-     if first usage of current is after nextUsePos[reg] then
+  let nextUsePos' :=
+      getRegisterIndex st (nextUseAfter pos) (const None) (active sd) in
+  let intersectingIntervals :=
+        filter (fun x => anyRangeIntersects
+                           (rds (curIntDesc cur))
+                           (rds (projT1 (getInterval sd x))))
+               (inactive sd) in
+  let nextUsePos :=
+      getRegisterIndex st (nextUseAfter pos)
+                       nextUsePos' intersectingIntervals in
+
+  (* reg = register with highest nextUsePos *)
+  let lastReg     := ultimate_from_nat maxReg registers_exist in
+  let (reg, mres) := findRegister nextUsePos lastReg in
+
+  (* if first usage of current is after nextUsePos[reg] then
        // all other intervals are used before current, so it is best
        // to spill current itself
        assign spill slot to current
@@ -939,13 +235,26 @@ Definition allocateBlockedReg `(cur : ScanStateCursor sd)
        current.reg = reg
        split active interval for reg at position
        split any inactive interval for reg at the end of its lifetime hole *)
+  let next :=
+      if (match mres with
+          | None   => false
+          | Some n => n <? pos
+          end)
+      then let next := assignSpillSlotToCurrent cur in
+           splitInterval cur undefined
+      else undefined in
 
   (* // make sure that current does not intersect with
      // the fixed interval for reg
      if current intersects with the fixed interval for reg then
        split current before this intersection *)
-
-  Build_NextScanState sd (curState cur) undefined.
+  let cursor := cursorFromMorphStLen cur next in
+  if true
+  (* then moveUnhandledToActive *)
+  (*          (cursorFromMorphStLen cursor (splitInterval cursor undefined)) reg *)
+  (* else next. *)
+  then undefined
+  else undefined.
 
 Fixpoint checkActiveIntervals `(st : ScanState sd) pos
   : NextScanState (SSMorphLen sd) :=
@@ -1083,6 +392,8 @@ Proof. intros; inversion smorph2; assumption. Defined.
 
 (** * Program graphs *)
 
+Definition VirtReg := nat.
+
 (** Given a node graph of our low-level intermediate representation, where
     instructions are associated with virtual registers, compute the linear
     mapping to intervals. *)
@@ -1093,10 +404,9 @@ Class Graph (a : Set) := {
 
 Definition determineIntervals (g : Graph VirtReg)
   : { sd : ScanStateDesc & ScanState sd }.
+  (* jww (2014-09-26): NYI *)
 Admitted.
 
 Definition allocateRegisters (g : Graph VirtReg)
   : { sd : ScanStateDesc & ScanState sd } :=
   let (sd,st) := determineIntervals g in linearScan sd st.
-
-End Allocator.
