Interval.v
@@ -1,0 +1,116 @@
+Require Import Lib.
+Require Import Range.
+
+Generalizable All Variables.
+
+(** ** Interval *)
+
+(** A lifetime interval defines the lifetime of a variable.  It is defined as
+    a list of ranges "covered" by that variable in the low-level intermediate
+    representation (LIR).  Gaps in the list of ranges are called "lifetime
+    holes".
+
+    A lifetime is not necessarily only the distance that a variable is first
+    and last used.  The lifetime of a variable used in a loop extends to the
+    whole loop, for example, even if it is only used at the very end.  In this
+    sense, coverage takes into account code flow, or what ranges would map to
+    if all loops were unrolled, and then rolled back keeping track of
+    coverage.
+
+    Use positions are actual instructions where a variable is read from or
+    written to, and whether it is required to be in a register at that
+    point. *)
+
+(** If for some reason we cannot assign a single register for all ranges, then
+    the interval is split into two or more intervals, so each interval can be
+    assigned its own register. *)
+
+Record IntervalDesc := {
+    ibeg : nat;
+    iend : nat;
+    rds  : NonEmpty RangeDesc;
+
+    (** Caching this property comes in handy, as it can be tricky to determine
+        it by reduction in some cases. *)
+    interval_nonempty : ibeg < iend
+}.
+
+Inductive Interval : IntervalDesc -> Set :=
+  | I_Sing : forall x, Range x ->
+      Interval {| ibeg := rbeg x
+                ; iend := rend x
+                ; rds  := NE_Sing x
+                ; interval_nonempty := range_nonempty x
+                |}
+
+  | I_Cons1 : forall x y ib ie ne,
+      Interval {| ibeg := ib; iend := ie; rds := NE_Sing y;
+                  interval_nonempty := ne |}
+        -> Range x -> forall (H : rend x <= ib),
+      Interval {| ibeg := rbeg x
+                ; iend := ie
+                ; rds  := NE_Cons x (NE_Sing y)
+                ; interval_nonempty := lt_le_shuffle (range_nonempty x) H ne
+                |}
+
+  | I_Consn : forall x y xs ib ie ne,
+      Interval {| ibeg := ib; iend := ie; rds := NE_Cons y xs;
+                  interval_nonempty := ne |}
+        -> Range x -> forall (H : rend x <= ib),
+      Interval {| ibeg := rbeg x
+                ; iend := ie
+                ; rds  := NE_Cons x (NE_Cons y xs)
+                ; interval_nonempty := lt_le_shuffle (range_nonempty x) H ne
+                |}.
+
+Definition intervalStart `(i : Interval d) : nat := ibeg d.
+Definition intervalEnd   `(i : Interval d) : nat := iend d.
+
+Definition intervalCoversPos `(i : Interval rs) (pos : nat) : bool :=
+  andb (intervalStart i <=? pos) (pos <? intervalEnd i).
+
+Definition intervalExtent `(i : Interval rs) :=
+  intervalEnd i - intervalStart i.
+
+Lemma Interval_nonempty : forall `(i : Interval rs),
+  intervalStart i < intervalEnd i.
+Proof.
+  intros. unfold intervalStart, intervalEnd.
+  induction i; simpl in *;
+  induction r; simpl in *; min_max.
+Qed.
+
+Lemma Interval_extent_nonzero : forall `(i : Interval rs),
+  intervalExtent i > 0.
+Proof.
+  intros.
+  unfold intervalExtent.
+  pose (Interval_nonempty i).
+  apply lt_minus in l. assumption.
+Qed.
+
+(** Fixed Intervals
+
+    Some machine instructions require their operands in fixed
+    registers. Such constraints are already considered during the
+    construction of the LIR by emitting physical register operands instead
+    of virtual register operands. Although the register allocator must
+    leave these operands unchanged, they must be considered during
+    register allocation because they limit the number of available
+    registers. Information about physical registers is collected in fixed
+    intervals.
+
+    For each physical register, one fixed interval stores where the
+    register is not available for allocation. Use positions are not needed
+    for fixed intervals because they are never split and spilled. Register
+    constraints at method calls are also modeled using fixed intervals:
+    Because all registers are destroyed when the call is executed, ranges
+    of length 1 are added to all fixed intervals at the call
+    site. Therefore, the allocation pass cannot assign a register to any
+    interval there, and all intervals are spilled before the call.
+
+    Note that we do not distinguish between the two types of intervals in this
+    code, and in fact make use of the use positions to track the locations of
+    fixity (such as call sites) within the code. *)
+
+Definition FixedInterval := Interval.
