Range.v
@@ -1,0 +1,95 @@
+Require Import Lib.
+
+(** ** UsePos *)
+
+(** A "use position", or [UsePos], identifies an exact point in the
+    instruction stream where a particular variable is used.  If this usage
+    requires the use of a physical register, then [regReq] is [true] for that
+    use position. *)
+
+Record UsePos : Set := {
+  uloc   : nat;
+  regReq : bool
+}.
+
+(** ** Range *)
+
+(** The extent of a [Range] is the set of locations it ranges over.  By
+    summing the extent of a list of ranges, we have an idea of how much ground
+    is left to cover, and this gives us a notion of well-founded recursion for
+    iterating over intervals that may split as we examine them -- i.e., whose
+    total extent must decrease after each pass.
+
+    A Range is built up from a set of use positions, and defines the inclusive
+    range of those positions.  It can be extended, or split, but never shrunk.
+    Also, the non-empty list of use positions is not guaranteed to be in any
+    order, and overlapping use positions are accepted but only the most recent
+    one "wins". *)
+
+Record RangeDesc := {
+    rbeg : nat;
+    rend : nat;
+    ups  : NonEmpty UsePos;
+
+    range_nonempty : rbeg < rend         (* this comes in handy *)
+}.
+
+Inductive Range : RangeDesc -> Set :=
+  | R_Sing u :
+    Range {| rbeg := uloc u
+           ; rend := S (uloc u)
+           ; ups  := NE_Sing u
+           ; range_nonempty := le_n (S (uloc u))
+           |}
+
+  | R_Cons u x : Range x -> forall (H : uloc u < rbeg x),
+    Range {| rbeg := uloc u
+           ; rend := rend x
+           ; ups  := NE_Cons u (ups x)
+           ; range_nonempty := Lt.lt_trans _ _ _ H (range_nonempty x)
+           |}
+
+  | R_Extend x b' e' : Range x ->
+    Range {| rbeg := min b' (rbeg x)
+           ; rend := Peano.max e' (rend x)
+           ; ups  := ups x
+           ; range_nonempty := min_lt_max _ _ _ _ (range_nonempty x)
+           |}.
+
+Definition rangeExtent (x : RangeDesc) := rend x - rbeg x.
+
+Definition rangesIntersect (x y : RangeDesc) : bool :=
+  if rbeg x <? rbeg y
+  then rbeg y <? rend x
+  else rbeg x <? rend y.
+
+Definition rangesIntersectionPoint (x y : RangeDesc) : option nat :=
+  if rangesIntersect x y
+  then Some (min (rbeg x) (rbeg y))
+  else None.
+
+Definition anyRangeIntersects (is js : NonEmpty RangeDesc) : bool :=
+  fold_right
+    (fun r b => orb b (existsb (rangesIntersect r) (NE_to_list js)))
+    false (NE_to_list is).
+
+Fixpoint NE_fold_left {a b : Set} (f : a -> b -> a) (ne : NonEmpty b) (z : a) : a :=
+  match ne with
+    | NE_Sing x => f z x
+    | NE_Cons x xs => NE_fold_left f xs (f z x)
+  end.
+
+Definition firstIntersectionPoint (rd1 rd2 : NonEmpty RangeDesc)
+  : option nat :=
+  NE_fold_left
+    (fun acc rd =>
+       match acc with
+       | Some x => Some x
+       | None =>
+         NE_fold_left
+           (fun acc' rd' =>
+              match acc' with
+              | Some x => Some x
+              | None => rangesIntersectionPoint rd rd'
+              end) rd2 None
+       end) rd1 None.
