ScanState.v
@@ -1,0 +1,657 @@
+Require Import Coq.Program.Tactics.
+Require Import Coq.Structures.Orders.
+Require Import Interval.
+Require Import Lib.
+
+Module Import LN := ListNotations.
+
+Generalizable All Variables.
+
+Module Type Machine.
+
+Variable maxReg : nat.          (* max number of registers *)
+
+Hypothesis registers_exist : maxReg > 0.
+
+End Machine.
+
+Module MScanState (M : Machine).
+Import M.
+
+Definition PhysReg := fin maxReg.
+Definition maxReg := maxReg.
+Definition registers_exist := registers_exist.
+
+(** ** ScanState *)
+
+(** A [ScanState] is always relative to a current position (pos) as we move
+    through the sequentialized instruction stream over which registers are
+    allocated.. *)
+
+Record ScanStateDesc := {
+    nextInterval : nat;
+    IntervalId   := fin nextInterval;
+
+    unhandled : list IntervalId;   (* starts after pos *)
+    active    : list IntervalId;   (* ranges over pos *)
+    inactive  : list IntervalId;   (* falls in lifetime hole *)
+    handled   : list IntervalId;   (* ends before pos *)
+
+    getInterval      : IntervalId -> { d : IntervalDesc & Interval d };
+    assignments      : IntervalId -> option PhysReg;
+
+    (** Fixed Intervals
+
+        Some machine instructions require their operands in fixed
+        registers. Such constraints are already considered during the
+        construction of the LIR by emitting physical register operands instead
+        of virtual register operands. Although the register allocator must
+        leave these operands unchanged, they must be considered during
+        register allocation because they limit the number of available
+        registers. Information about physical registers is collected in fixed
+        intervals.
+
+        For each physical register, one fixed interval stores where the
+        register is not available for allocation. Use positions are not needed
+        for fixed intervals because they are never split and spilled. Register
+        constraints at method calls are also modeled using fixed intervals:
+        Because all registers are destroyed when the call is executed, ranges
+        of length 1 are added to all fixed intervals at the call
+        site. Therefore, the allocation pass cannot assign a register to any
+        interval there, and all intervals are spilled before the call. *)
+
+    getFixedInterval : PhysReg -> option { d : IntervalDesc & FixedInterval d };
+
+    (* jww (2014-09-25): These restricting lemmas should be added back once
+       everything is functional. *)
+    (* unhandled_sorted : StronglySorted cmp_le unhandled; *)
+
+    all_state_lists  := unhandled ++ active ++ inactive ++ handled;
+    lists_are_unique : NoDup all_state_lists
+}.
+
+Lemma lt_sub : forall n m, n < m -> { p : nat | p = m - n }.
+Proof. intros. exists (m - n). reflexivity. Defined.
+
+Definition transportId `(H : nextInterval st <= nextInterval st')
+  (x : IntervalId st) : IntervalId st'.
+Proof.
+  apply Compare_dec.le_lt_eq_dec in H.
+  destruct H.
+    destruct st. destruct st'.
+    unfold IntervalId0, IntervalId1 in *.
+    unfold IntervalId in *. simpl in *.
+    pose proof l.
+    apply lt_sub in H.
+    destruct H.
+    symmetry in e.
+    apply Nat.add_sub_eq_nz in e.
+      rewrite Plus.plus_comm in e.
+      rewrite <- e.
+      apply (R x0 x).
+    subst. omega.
+  unfold IntervalId in *.
+  rewrite <- e.
+  assumption.
+Defined.
+
+Lemma move_unhandled_to_active : forall n (x : fin n) unh act inact hnd,
+  NoDup ((x :: unh) ++ act ++ inact ++ hnd)
+    -> NoDup (unh ++ (x :: act) ++ inact ++ hnd).
+Proof.
+  intros. rewrite <- app_comm_cons.
+  apply NoDup_app_cons. assumption.
+Qed.
+
+Lemma move_active_to_inactive : forall sd x,
+  NoDup (unhandled sd ++ active sd ++ inactive sd ++ handled sd)
+    -> In x (active sd)
+    -> NoDup (unhandled sd ++ remove cmp_eq_dec x (active sd) ++
+              (x :: inactive sd) ++ handled sd).
+Proof.
+  intros.
+  apply NoDup_swap.
+  rewrite <- app_assoc.
+  rewrite <- app_assoc.
+  apply NoDup_juggle.
+  rewrite app_assoc.
+  rewrite app_assoc.
+  apply NoDup_swap.
+  rewrite <- app_assoc.
+  assumption.
+  apply H0.
+Qed.
+
+Lemma move_active_to_handled : forall sd x,
+  NoDup (unhandled sd ++ active sd ++ inactive sd ++ handled sd)
+    -> In x (active sd)
+    -> NoDup (unhandled sd ++ remove cmp_eq_dec x (active sd) ++
+              inactive sd ++ x :: handled sd).
+Proof.
+  intros.
+  apply NoDup_swap.
+  rewrite <- app_assoc.
+  rewrite <- app_assoc.
+  apply NoDup_swap2.
+  rewrite <- app_assoc.
+  apply NoDup_juggle.
+  rewrite app_assoc.
+  apply NoDup_swap2.
+  rewrite app_assoc.
+  apply NoDup_swap.
+  rewrite <- app_assoc.
+  rewrite app_assoc.
+  apply NoDup_swap2.
+  rewrite <- app_assoc.
+  assumption.
+  apply H0.
+Qed.
+
+Lemma move_inactive_to_active : forall sd x,
+  NoDup (unhandled sd ++ active sd ++ inactive sd ++ handled sd)
+    -> In x (inactive sd)
+    -> NoDup (unhandled sd ++ x :: active sd ++
+              remove cmp_eq_dec x (inactive sd) ++ handled sd).
+Proof.
+  intros.
+  rewrite app_comm_cons.
+  apply NoDup_swap.
+  rewrite <- app_assoc.
+  apply NoDup_swap.
+  repeat rewrite <- app_assoc.
+  rewrite (app_assoc (handled sd)).
+  apply NoDup_swap2.
+  apply NoDup_juggle.
+  repeat rewrite app_assoc.
+  apply NoDup_swap.
+  rewrite <- app_assoc.
+  apply NoDup_swap2.
+  rewrite <- app_assoc.
+  rewrite app_assoc.
+  apply NoDup_swap2.
+  rewrite <- app_assoc.
+  assumption.
+  apply H0.
+Qed.
+
+Lemma move_inactive_to_handled : forall sd x,
+  NoDup (unhandled sd ++ active sd ++ inactive sd ++ handled sd)
+    -> In x (inactive sd)
+    -> NoDup (unhandled sd ++ active sd ++
+              remove cmp_eq_dec x (inactive sd) ++ x :: handled sd).
+Proof.
+  intros.
+  rewrite (app_assoc (unhandled sd)).
+  apply NoDup_swap.
+  repeat rewrite <- app_assoc.
+  apply NoDup_juggle.
+  rewrite (app_assoc (inactive sd)).
+  apply NoDup_swap.
+  repeat rewrite <- app_assoc.
+  assumption.
+  apply H0.
+Qed.
+
+(** The [ScanState] inductive data type describes the allowable state
+    transitions that can be applied to a [ScanStateDesc] value.
+
+    In essence there are five mutating operations:
+
+    1. Create a new unhandled interval.  This can occur for two reasons:
+
+       a. Adding a new interval to be considered before the linear scan
+          algorithm has started.
+       b. Splitting the current interval, which pushes back its "pieces" as
+          new unhandled intervals.
+
+    2. Remove the first unhandled interval.  This happens when we remove it in
+       order to make it the new current interval.
+
+    3. Add the current interval to the active list.
+
+    4. Move an item from the active list to the inactive or handled lists.
+
+    5. Move an item from the inactive list to the active or handled lists. *)
+
+Inductive ScanState : ScanStateDesc -> Set :=
+  | ScanState_nil :
+    ScanState
+      {| nextInterval     := 0
+       ; unhandled        := nil
+       ; active           := nil
+       ; inactive         := nil
+       ; handled          := nil
+       ; getInterval      := fin_contra
+       ; assignments      := fin_contra
+       ; getFixedInterval := const None
+       (* ; unhandled_sorted := LSorted_nil _ *)
+       ; lists_are_unique := NoDup_nil _
+       |}
+
+  | ScanState_newUnhandled
+      ni unh (* unhsort *) act inact hnd geti assgn getfixi lau :
+    forall `(i : Interval d),
+    ScanState
+      {| nextInterval     := ni
+       ; unhandled        := unh
+       ; active           := act
+       ; inactive         := inact
+       ; handled          := hnd
+       ; getInterval      := geti
+       ; assignments      := assgn
+       ; getFixedInterval := getfixi
+       (* ; unhandled_sorted := unhsort *)
+       ; lists_are_unique := lau
+       |} ->
+    forall newi (H : newi = last_fin_from_nat ni),
+    ScanState
+      {| nextInterval     := S ni
+       ; unhandled        := newi :: map fin_expand unh
+       ; active           := map fin_expand act
+       ; inactive         := map fin_expand inact
+       ; handled          := map fin_expand hnd
+       ; getInterval      :=
+         fun n => match cmp_eq_dec n newi with
+                  | left _ => existT _ d i
+                  | right Hn => geti (fin_safe_reduce n (rew_in_not_eq H Hn))
+                  end
+       ; assignments      :=
+         fun n => match cmp_eq_dec n newi with
+                  | left _ => None
+                  | right Hn => assgn (fin_safe_reduce n (rew_in_not_eq H Hn))
+                  end
+       ; getFixedInterval := getfixi
+       (* ; unhandled_sorted := unhsort *)
+       ; lists_are_unique := map_fin_expand_rewrite (NoDup_fin_cons _ _ lau H)
+       |}
+
+  | ScanState_moveUnhandledToActive
+      ni unh (* unhsort *) act inact hnd geti assgn getfixi x reg :
+    forall lau : NoDup ((x :: unh) ++ act ++ inact ++ hnd),
+    ScanState
+      {| nextInterval     := ni
+       ; unhandled        := x :: unh
+       ; active           := act
+       ; inactive         := inact
+       ; handled          := hnd
+       ; getInterval      := geti
+       ; assignments      := assgn
+       ; getFixedInterval := getfixi
+       (* ; unhandled_sorted := unhandled_sorted sd *)
+       ; lists_are_unique := lau
+       |} ->
+    ScanState
+      {| nextInterval     := ni
+       ; unhandled        := unh
+       ; active           := x :: act
+       ; inactive         := inact
+       ; handled          := hnd
+       ; getInterval      := geti
+       ; assignments      := fun i => if cmp_eq_dec i x
+                                      then Some reg
+                                      else assgn i
+       ; getFixedInterval := getfixi
+       (* ; unhandled_sorted := unhandled_sorted sd *)
+       ; lists_are_unique := move_unhandled_to_active _ x unh act inact hnd lau
+       |}
+
+  | ScanState_moveActiveToInactive sd x :
+    ScanState sd -> forall (H : In x (active sd)),
+    ScanState
+      {| nextInterval     := nextInterval sd
+       ; unhandled        := unhandled sd
+       ; active           := remove cmp_eq_dec x (active sd)
+       ; inactive         := x :: inactive sd
+       ; handled          := handled sd
+       ; getInterval      := getInterval sd
+       ; assignments      := assignments sd
+       ; getFixedInterval := getFixedInterval sd
+       (* ; unhandled_sorted := unhandled_sorted sd *)
+       ; lists_are_unique :=
+         move_active_to_inactive sd x (lists_are_unique sd) H
+       |}
+
+  | ScanState_moveActiveToHandled sd x :
+    ScanState sd -> forall (H : In x (active sd)),
+    ScanState
+      {| nextInterval     := nextInterval sd
+       ; unhandled        := unhandled sd
+       ; active           := remove cmp_eq_dec x (active sd)
+       ; inactive         := inactive sd
+       ; handled          := x :: handled sd
+       ; getInterval      := getInterval sd
+       ; assignments      := assignments sd
+       ; getFixedInterval := getFixedInterval sd
+       (* ; unhandled_sorted := unhandled_sorted sd *)
+       ; lists_are_unique :=
+         move_active_to_handled sd x (lists_are_unique sd) H
+       |}
+
+  | ScanState_moveInactiveToActive sd x :
+    ScanState sd -> forall (H : In x (inactive sd)),
+    ScanState
+      {| nextInterval     := nextInterval sd
+       ; unhandled        := unhandled sd
+       ; active           := x :: active sd
+       ; inactive         := remove cmp_eq_dec x (inactive sd)
+       ; handled          := handled sd
+       ; getInterval      := getInterval sd
+       ; assignments      := assignments sd
+       ; getFixedInterval := getFixedInterval sd
+       (* ; unhandled_sorted := unhandled_sorted sd *)
+       ; lists_are_unique :=
+         move_inactive_to_active sd x (lists_are_unique sd) H
+       |}
+
+  | ScanState_moveInactiveToHandled sd x :
+    ScanState sd -> forall (H : In x (inactive sd)),
+    ScanState
+      {| nextInterval     := nextInterval sd
+       ; unhandled        := unhandled sd
+       ; active           := active sd
+       ; inactive         := remove cmp_eq_dec x (inactive sd)
+       ; handled          := x :: handled sd
+       ; getInterval      := getInterval sd
+       ; assignments      := assignments sd
+       ; getFixedInterval := getFixedInterval sd
+       (* ; unhandled_sorted := unhandled_sorted sd *)
+       ; lists_are_unique :=
+         move_inactive_to_handled sd x (lists_are_unique sd) H
+       |}.
+
+Tactic Notation "ScanState_cases" tactic(first) ident(c) :=
+  first;
+  [ Case_aux c "ScanState_nil"
+  | Case_aux c "ScanState_newUnhandled"
+  | Case_aux c "ScanState_moveUnhandledToActive"
+  | Case_aux c "ScanState_moveActiveToInactive"
+  | Case_aux c "ScanState_moveActiveToHandled"
+  | Case_aux c "ScanState_moveInactiveToActive"
+  | Case_aux c "ScanState_moveInactiveToHandled"
+  ].
+
+Ltac cmp_reflexive :=
+  match goal with
+    [ |- context [match cmp_eq_dec ?X ?X with _ => _ end] ] =>
+      assert (cmp_eq_dec X X = left eq_refl) as Hrcmp
+        by (intros; destruct (cmp_eq_dec X X);
+              [ f_equal; apply proof_irrelevance
+              | intuition ]);
+      rewrite Hrcmp in *; clear Hrcmp; simpl in *
+  end.
+
+Definition unhandledExtent `(sd : ScanStateDesc) : nat :=
+  match unhandled sd with
+  | nil => 0
+  | [i] => intervalExtent (projT2 (getInterval sd i))
+  | xs  =>
+    let f n x := n + intervalExtent (projT2 (getInterval sd x)) in
+    fold_left f xs 0
+  end.
+
+Theorem ScanState_unhandledExtent `(st : ScanState sd) :
+  let unh := unhandled sd in
+  let ue  := unhandledExtent sd in
+  match unh with
+  | nil    => ue = 0
+  | [i]    => ue = intervalExtent (projT2 (getInterval sd i))
+  | i :: _ => ue > intervalExtent (projT2 (getInterval sd i))
+  end.
+Proof.
+  destruct sd.
+  destruct unhandled0 eqn:Heqe;
+  unfold unhandledExtent; simpl.
+    reflexivity.
+  destruct l eqn:Heqe2; simpl.
+    reflexivity.
+  apply fold_gt.
+  pose (Interval_extent_nonzero (projT2 (getInterval0 i0))).
+  omega.
+Defined.
+
+Lemma unhandledExtent_cons
+  : forall ni i (unh : list (fin ni)) geti assgn assgn' getfixi
+           (act act' inact inact' hnd hnd' : list (fin ni))
+           (lau : NoDup (unh ++ act ++ inact ++ hnd))
+           (lau' : NoDup ((i :: unh) ++ act' ++ inact' ++ hnd')),
+  unhandledExtent
+    {| nextInterval     := ni
+     ; unhandled        := unh
+     ; active           := act
+     ; inactive         := inact
+     ; handled          := hnd
+     ; getInterval      := geti
+     ; assignments      := assgn
+     ; getFixedInterval := getfixi
+     ; lists_are_unique := lau
+     |} <
+  unhandledExtent
+    {| nextInterval     := ni
+     ; unhandled        := i :: unh
+     ; active           := act'
+     ; inactive         := inact'
+     ; handled          := hnd'
+     ; getInterval      := geti
+     ; assignments      := assgn'
+     ; getFixedInterval := getfixi
+     ; lists_are_unique := lau'
+     |}.
+Proof.
+  intros.
+  induction unh; unfold unhandledExtent; simpl;
+  pose (Interval_extent_nonzero (projT2 (geti i))). omega.
+  destruct unh; simpl. omega.
+  apply fold_fold_lt. omega.
+Qed.
+
+Record ScanStateCursor (sd : ScanStateDesc) := {
+    curState    : ScanState sd;
+    curExists   : length (unhandled sd) > 0;
+
+    curId       := safe_hd (unhandled sd) curExists;
+
+    curIntDesc  : IntervalDesc;
+    curInterval := projT2 (getInterval sd curId);
+
+    curPosition := intervalStart curInterval
+}.
+
+Arguments curState    {sd} _.
+Arguments curExists   {sd} _.
+Arguments curId       {sd} _.
+Arguments curIntDesc  {sd} _.
+Arguments curInterval {sd} _.
+Arguments curPosition {sd} _.
+
+Record NextScanState (P : ScanStateDesc -> Prop) : Type := {
+    nextDesc   : ScanStateDesc;
+    nextState  : ScanState nextDesc;
+    morphProof : P nextDesc
+}.
+
+Arguments Build_NextScanState [P] _ _ _.
+
+Arguments nextDesc   [P] _.
+Arguments nextState  [P] _.
+Arguments morphProof [P] _.
+
+Definition NextState `(cur : ScanStateCursor sd) P := NextScanState (P sd).
+
+Definition NextStateDep  `(cur : ScanStateCursor sd) P Q :=
+  { x : NextScanState (P sd) & Q x }.
+
+Definition NextStateWith `(cur : ScanStateCursor sd) P A :=
+  (A * NextScanState (P sd))%type.
+
+Definition NextScanState_transitivity
+  {P : ScanStateDesc -> ScanStateDesc -> Prop} `{Transitive _ P}
+  `(n : NextScanState (P sd0)) `(o : NextScanState (P (nextDesc n)))
+  : NextScanState (P sd0).
+  destruct n. destruct o.
+  simpl in *.
+  rapply Build_NextScanState.
+    apply nextState1.
+  transitivity nextDesc0; assumption.
+Defined.
+
+(** ** SSMorph *)
+
+(** A [SSMorph] is a relation describe a lawful transition between two
+    states.  It is a [PreOrder] relation. *)
+
+Record SSMorph (sd1 sd2 : ScanStateDesc) : Prop := {
+    next_interval_increases : nextInterval sd1     <= nextInterval sd2;
+    total_extent_decreases  : unhandledExtent sd2  <= unhandledExtent sd1;
+    handled_count_increases : length (handled sd1) <= length (handled sd2)
+}.
+
+Arguments next_interval_increases [sd1 sd2] _.
+Arguments total_extent_decreases  [sd1 sd2] _.
+Arguments handled_count_increases [sd1 sd2] _.
+
+Definition newSSMorph (s : ScanStateDesc) : SSMorph s s.
+Proof. constructor; auto. Defined.
+
+Program Instance SSMorph_PO : PreOrder SSMorph.
+Obligation 1. constructor; auto. Defined.
+Obligation 2.
+  constructor; destruct H; destruct H0.
+  transitivity (nextInterval y); auto.
+  transitivity (unhandledExtent y); auto.
+  transitivity (length (handled y)); auto.
+Defined.
+
+Record SSMorphLen (sd1 sd2 : ScanStateDesc) : Prop := {
+    len_is_SSMorph :> SSMorph sd1 sd2;
+
+    unhandled_nonempty :
+      length (unhandled sd1) > 0 -> length (unhandled sd2) > 0
+}.
+
+Definition newSSMorphLen (s : ScanStateDesc) : SSMorphLen s s.
+Proof. intros. constructor; auto. constructor; auto. Defined.
+
+Record SSMorphSt (sd1 sd2 : ScanStateDesc) : Prop := {
+    st_is_SSMorph :> SSMorph sd1 sd2;
+
+    total_extent_measurably_decreases :
+      unhandledExtent sd2 < unhandledExtent sd1
+}.
+
+Program Instance SSMorphSt_Trans : Transitive SSMorphSt.
+Obligation 1.
+  constructor.
+    destruct H. destruct H0.
+    transitivity y; assumption.
+  inversion H. inversion H0.
+  destruct total_extent_measurably_decreases1. omega.
+  destruct total_extent_measurably_decreases0. omega.
+  right. omega.
+Qed.
+
+Record SSMorphStLen (sd1 sd2 : ScanStateDesc) : Prop := {
+    stlen_is_SSMorphLen :> SSMorphLen sd1 sd2;
+    stlen_is_SSMorphSt  :> SSMorphSt sd1 sd2
+}.
+
+Lemma ScanState_unhandledExtent_nonzero `(st : ScanState sd) :
+  length (unhandled sd) > 0 <-> unhandledExtent sd > 0.
+Proof.
+  intros.
+  ScanState_cases (induction st) Case; simpl in *.
+  - Case "ScanState_nil".
+    split; intros; inversion H.
+  - Case "ScanState_newUnhandled".
+    pose (Interval_extent_nonzero i).
+    destruct unh eqn:Heqe;
+    unfold unhandledExtent; simpl.
+      split; intros; try cmp_reflexive; auto.
+    destruct l eqn:Heqe2; simpl.
+      split; intros; try cmp_reflexive; auto. omega.
+    split; intros.
+      apply fold_gt.
+      cmp_reflexive. omega.
+    apply Gt.gt_Sn_O.
+  - Case "ScanState_moveUnhandledToActive".
+    apply ScanState_unhandledExtent in st.
+    rename st into i. simpl in *.
+    destruct unh eqn:Heqe.
+      split; intros. inversion H. auto.
+    unfold unhandledExtent; simpl.
+    destruct l eqn:Heqe2; simpl.
+      split; intros.
+      apply Interval_extent_nonzero.
+      auto.
+    split; intros.
+      apply fold_gt.
+      pose (Interval_extent_nonzero (projT2 (geti f))).
+      omega.
+    omega.
+  - Case "ScanState_moveActiveToInactive".  apply IHst.
+  - Case "ScanState_moveActiveToHandled".   apply IHst.
+  - Case "ScanState_moveInactiveToActive".  apply IHst.
+  - Case "ScanState_moveInactiveToHandled". apply IHst.
+Qed.
+
+Definition moveActiveToHandled `(st : ScanState sd) (x : IntervalId sd)
+  (H : In x (active sd)) : NextScanState (SSMorphLen sd).
+Proof.
+  pose (ScanState_moveActiveToInactive sd x st H). eexists. apply s.
+  destruct sd. simpl.
+  rapply Build_SSMorphLen; auto.
+  rapply Build_SSMorph; auto.
+Defined.
+
+Definition moveActiveToInactive `(st : ScanState sd) (x : IntervalId sd)
+  (H : In x (active sd)) : NextScanState (SSMorphLen sd).
+Proof.
+  pose (ScanState_moveActiveToInactive sd x st H). eexists. apply s.
+  destruct sd. simpl.
+  rapply Build_SSMorphLen; auto.
+  rapply Build_SSMorph; auto.
+Defined.
+
+Definition moveInactiveToActive `(st : ScanState sd) (x : IntervalId sd)
+  (H : In x (inactive sd)) : NextScanState (SSMorphLen sd).
+Proof.
+  pose (ScanState_moveInactiveToActive sd x st H). eexists. apply s.
+  destruct sd. simpl.
+  rapply Build_SSMorphLen; auto.
+  rapply Build_SSMorph; auto.
+Defined.
+
+Definition moveInactiveToHandled `(st : ScanState sd) (x : IntervalId sd)
+  (H : In x (inactive sd)) : NextScanState (SSMorphLen sd).
+Proof.
+  pose (ScanState_moveInactiveToHandled sd x st H). eexists. apply s.
+  destruct sd. simpl.
+  rapply Build_SSMorphLen; auto.
+  rapply Build_SSMorph; auto.
+  apply Le.le_n_Sn.
+Defined.
+
+Definition moveUnhandledToActive `(cur : ScanStateCursor sd) (reg : PhysReg)
+  : NextState cur SSMorphSt.
+Proof.
+  destruct cur. destruct sd.
+  destruct unhandled0; simpl in *. omega.
+  pose (ScanState_moveUnhandledToActive nextInterval0 unhandled0
+          (* unhsort *)
+          active0 inactive0 handled0 getInterval0 assignments0
+          getFixedInterval0 i reg lists_are_unique0).
+  eexists. apply s. apply curState0.
+  pose (unhandledExtent_cons nextInterval0 i unhandled0 getInterval0
+         (fun i0 : fin nextInterval0 =>
+            if cmp_eq_dec i0 i
+            then Some reg
+            else assignments0 i0) assignments0 getFixedInterval0
+         (i :: active0) active0 inactive0 inactive0 handled0 handled0
+         (move_unhandled_to_active _ i unhandled0 active0 inactive0 handled0
+            lists_are_unique0) lists_are_unique0)
+    as ue_cons.
+  rapply Build_SSMorphSt; auto.
+  rapply Build_SSMorph; auto.
+  apply (Lt.lt_le_weak _ _ ue_cons).
+Defined.
+
+End MScanState.
